use global target ident

stanfrontend/Target.v
@@ -114,17 +114,7 @@ Fixpoint transf_starget_statement (s: CStan.statement) {struct s}: res CStan.sta
   | Stilde e i le (oe0, oe1) => Error (msg "Stilde DNE in this stage of pipeline")
 end.
 
-Notation localvar := (prod AST.ident Ctypes.type).
-
-(* assuming that target is always symbol 0 to a model lets us remove this hack *)
-Definition get_target_ident (vars: list localvar) : res AST.ident :=
-  match vars with
-  | nil => Error (msg "impossible: 0")
-  | (t, ty)::_ => OK t
-  (* | _ => error (msg "impossible: >1") *)
-  end.
-
-Fixpoint transf_etarget_expr (tgt: AST.ident) (e: CStan.expr) {struct e}: res CStan.expr :=
+Fixpoint transf_etarget_expr (ot : AST.ident) (e: CStan.expr) {struct e}: res CStan.expr :=
   match e with
   | CStan.Econst_int i t => OK (CStan.Econst_int i t)
   | CStan.Econst_float f t => OK (CStan.Econst_float f t)
@@ -133,64 +123,67 @@ Fixpoint transf_etarget_expr (tgt: AST.ident) (e: CStan.expr) {struct e}: res CS
   | CStan.Evar i t => OK (CStan.Evar i t)
   | CStan.Etempvar i t => OK (CStan.Etempvar i t)
   | CStan.Ederef e t =>
-    do e <- transf_etarget_expr tgt e;
+    do e <- transf_etarget_expr ot e;
     OK (CStan.Ederef e t)
   | CStan.Ecast e t => OK (CStan.Ecast e t)
   | CStan.Efield e i t => OK (CStan.Efield e i t)
   | CStan.Eunop uop e t =>
-    do e <- transf_etarget_expr tgt e;
+    do e <- transf_etarget_expr ot e;
     OK (CStan.Eunop uop e t)
   | CStan.Ebinop bop e0 e1 t =>
-    do e0 <- transf_etarget_expr tgt e0;
-    do e1 <- transf_etarget_expr tgt e1;
+    do e0 <- transf_etarget_expr ot e0;
+    do e1 <- transf_etarget_expr ot e1;
     OK (CStan.Ebinop bop e0 e1 t)
   | CStan.Eaddrof e t => OK (CStan.Eaddrof e t)
   | CStan.Esizeof t0 t1 => OK (CStan.Esizeof t0 t1)
   | CStan.Ealignof t0 t1 => OK (CStan.Ealignof t0 t1)
-  | CStan.Etarget ty => OK (CStan.Evar tgt ty)
+  | CStan.Etarget ty => OK (CStan.Evar ot ty)
 end.
 
-Fixpoint transf_etarget_statement (tgt: AST.ident) (s: CStan.statement) {struct s}: res CStan.statement :=
+Fixpoint transf_etarget_statement (t : AST.ident) (s: CStan.statement) {struct s}: res CStan.statement :=
 match s with
   | Sassign e0 e1 =>
-    do e0 <- transf_etarget_expr tgt e0;
-    do e1 <- transf_etarget_expr tgt e1;
+    do e0 <- transf_etarget_expr t e0;
+    do e1 <- transf_etarget_expr t e1;
     OK (Sassign e0 e1)
-  | Sset i e => do e <- transf_etarget_expr tgt e; OK (Sset i e)
+  | Sset i e =>
+    do e <- transf_etarget_expr t e;
+    if Pos.eqb i t
+    then Error (msg "cannot set the target identifier")
+    else OK (Sset i e)
   | Scall oi e le =>
-    do e <- transf_etarget_expr tgt e;
-    do le <- res_mmap (transf_etarget_expr tgt) le;
+    do e <- transf_etarget_expr t e;
+    do le <- res_mmap (transf_etarget_expr t) le;
     OK (Scall oi e le)
   | Sbuiltin oi ef lt le => Error (msg "ret (Sbuiltin oi ef lt le)")
   | Ssequence s0 s1 =>
-    do s0 <- transf_etarget_statement tgt s0;
-    do s1 <- transf_etarget_statement tgt s1;
+    do s0 <- transf_etarget_statement t s0;
+    do s1 <- transf_etarget_statement t s1;
     OK (Ssequence s0 s1)
   | Sifthenelse e s0 s1 =>
-    do e <- transf_etarget_expr tgt e;
-    do s0 <- transf_etarget_statement tgt s0;
-    do s1 <- transf_etarget_statement tgt s1;
+    do e <- transf_etarget_expr t e;
+    do s0 <- transf_etarget_statement t s0;
+    do s1 <- transf_etarget_statement t s1;
     OK (Sifthenelse e s0 s1)
   | Sloop s0 s1 =>
-    do s0 <- transf_etarget_statement tgt s0;
-    do s1 <- transf_etarget_statement tgt s1;
+    do s0 <- transf_etarget_statement t s0;
+    do s1 <- transf_etarget_statement t s1;
     OK (Sloop s0 s1)
   | Sreturn oe =>
-    do oe <- option_res_mmap (transf_etarget_expr tgt) oe;
+    do oe <- option_res_mmap (transf_etarget_expr t) oe;
     OK (Sreturn oe)
   | Starget e =>
     Error (msg "Starget DNE in this stage of pipeline")
   | Stilde e i le (oe0, oe1) =>
     Error (msg "Stilde DNE in this stage of pipeline")
-
   | Sbreak => OK Sbreak
   | Sskip => OK Sskip
   | Scontinue => OK Scontinue
 end.
 
-Definition transf_model_statement (tgt: AST.ident) (body: statement) :res CStan.statement :=
+Definition transf_statement (t: AST.ident) (body: statement) : res CStan.statement :=
   do body <- transf_starget_statement body;
-  transf_etarget_statement tgt body.
+  transf_etarget_statement t body.
 
 Definition add_prelude_epilogue (body: statement) : CStan.statement :=
   let tytarget := tdouble in
@@ -198,12 +191,15 @@ Definition add_prelude_epilogue (body: statement) : CStan.statement :=
   let epilogue := Sreturn (Some (CStan.Etarget tytarget)) in
   Ssequence prelude (Ssequence body epilogue).
 
-Definition transf_function (f: function): res function :=
-  match f.(fn_blocktype) with
-  | BTModel =>
-    do tgt <- get_target_ident f.(fn_vars);
-    do body <- transf_model_statement tgt (add_prelude_epilogue f.(fn_body));
-    OK {|
+Definition transf_model_body (f: function): statement :=
+match f.(fn_blocktype) with
+| BTModel => add_prelude_epilogue f.(fn_body)
+| _ => f.(fn_body)
+end.
+
+Definition transf_function (tgt: AST.ident) (f: function): res function :=
+  do body <- transf_statement tgt (transf_model_body f);
+  OK {|
       fn_params := f.(fn_params);
       fn_body := body;
 
@@ -215,9 +211,7 @@ Definition transf_function (f: function): res function :=
       fn_return := f.(fn_return);
       fn_callconv := f.(fn_callconv);
       fn_blocktype := f.(fn_blocktype);
-     |}
-  | _ => OK f
-  end.
+     |}.
 
 Definition transf_external (ef: AST.external_function) : res AST.external_function :=
   match ef with
@@ -226,17 +220,17 @@ Definition transf_external (ef: AST.external_function) : res AST.external_functi
   | _ => OK ef
   end.
 
-Definition transf_fundef (fd: CStan.fundef) : res CStan.fundef :=
+Definition transf_fundef (tgt: AST.ident) (fd: CStan.fundef) : res CStan.fundef :=
   match fd with
-  | Internal f => do tf <- transf_function f; OK (Internal tf)
+  | Internal f => do tf <- transf_function tgt f; OK (Internal tf)
   | External ef targs tres cc => do ef <- transf_external ef; OK (External ef targs tres cc)
   end.
 
 Definition transf_variable (v: type): res type :=
   OK v.
 
-Definition transf_program(p: CStan.program): res CStan.program :=
-  do p1 <- AST.transform_partial_program2 (fun i => transf_fundef) (fun i => transf_variable) p;
+Definition transf_program (p: CStan.program): res CStan.program :=
+  do p1 <- AST.transform_partial_program2 (fun i => transf_fundef p.(prog_target)) (fun i => transf_variable) p;
   OK {|
       prog_defs := AST.prog_defs p1;
       prog_public := AST.prog_public p1;
@@ -254,7 +248,7 @@ Definition transf_program(p: CStan.program): res CStan.program :=
 
       prog_generated_quantities:=p.(prog_generated_quantities);
       prog_model:=p.(prog_model);
-
+      prog_target:=p.(prog_target);
       prog_main:=p.(prog_main);
 
       prog_types:=p.(prog_types);
@@ -264,100 +258,3 @@ Definition transf_program(p: CStan.program): res CStan.program :=
       prog_math_functions:= p.(prog_math_functions);
       prog_dist_functions:= p.(prog_dist_functions);
     |}.
-
-(*******************************************************************)
-
-Fixpoint transf_etarget_expr_alt (ot : option AST.ident) (e: CStan.expr) {struct e}: res CStan.expr :=
-  match e with
-  | CStan.Econst_int i t => OK (CStan.Econst_int i t)
-  | CStan.Econst_float f t => OK (CStan.Econst_float f t)
-  | CStan.Econst_single f t => OK (CStan.Econst_single f t)
-  | CStan.Econst_long i t => OK (CStan.Econst_long i t)
-  | CStan.Evar i t => OK (CStan.Evar i t)
-  | CStan.Etempvar i t => OK (CStan.Etempvar i t)
-  | CStan.Ederef e t =>
-    do e <- transf_etarget_expr_alt ot e;
-    OK (CStan.Ederef e t)
-  | CStan.Ecast e t => OK (CStan.Ecast e t)
-  | CStan.Efield e i t => OK (CStan.Efield e i t)
-  | CStan.Eunop uop e t =>
-    do e <- transf_etarget_expr_alt ot e;
-    OK (CStan.Eunop uop e t)
-  | CStan.Ebinop bop e0 e1 t =>
-    do e0 <- transf_etarget_expr_alt ot e0;
-    do e1 <- transf_etarget_expr_alt ot e1;
-    OK (CStan.Ebinop bop e0 e1 t)
-  | CStan.Eaddrof e t => OK (CStan.Eaddrof e t)
-  | CStan.Esizeof t0 t1 => OK (CStan.Esizeof t0 t1)
-  | CStan.Ealignof t0 t1 => OK (CStan.Ealignof t0 t1)
-  | CStan.Etarget ty =>
-    match ot with
-    | None => Error (msg "impossible: etarget transformation called out of order in compiler phases")
-    | Some tgt => OK (CStan.Evar tgt ty)
-    end
-end.
-
-Fixpoint transf_etarget_statement_alt (ot : option AST.ident) (s: CStan.statement) {struct s}: res CStan.statement :=
-match s with
-  | Sassign e0 e1 =>
-    do e0 <- transf_etarget_expr_alt ot e0;
-    do e1 <- transf_etarget_expr_alt ot e1;
-    OK (Sassign e0 e1)
-  | Sset i e => do e <- transf_etarget_expr_alt ot e; OK (Sset i e)
-  | Scall oi e le =>
-    do e <- transf_etarget_expr_alt ot e;
-    do le <- res_mmap (transf_etarget_expr_alt ot) le;
-    OK (Scall oi e le)
-  | Sbuiltin oi ef lt le => Error (msg "ret (Sbuiltin oi ef lt le)")
-  | Ssequence s0 s1 =>
-    do s0 <- transf_etarget_statement_alt ot s0;
-    do s1 <- transf_etarget_statement_alt ot s1;
-    OK (Ssequence s0 s1)
-  | Sifthenelse e s0 s1 =>
-    do e <- transf_etarget_expr_alt ot e;
-    do s0 <- transf_etarget_statement_alt ot s0;
-    do s1 <- transf_etarget_statement_alt ot s1;
-    OK (Sifthenelse e s0 s1)
-  | Sloop s0 s1 =>
-    do s0 <- transf_etarget_statement_alt ot s0;
-    do s1 <- transf_etarget_statement_alt ot s1;
-    OK (Sloop s0 s1)
-  | Sreturn oe =>
-    do oe <- option_res_mmap (transf_etarget_expr_alt ot) oe;
-    OK (Sreturn oe)
-  | Starget e =>
-    Error (msg "Starget DNE in this stage of pipeline")
-  | Stilde e i le (oe0, oe1) =>
-    Error (msg "Stilde DNE in this stage of pipeline")
-  | Sbreak => OK Sbreak
-  | Sskip => OK Sskip
-  | Scontinue => OK Scontinue
-end.
-
-Definition transf_statement_alt (ot: option AST.ident) (body: statement) : res CStan.statement :=
-  do body <- transf_starget_statement body;
-  transf_etarget_statement_alt ot body.
-
-Definition transf_function_body_alt (f: function): res statement :=
-match f.(fn_blocktype) with
-| BTModel =>
-  do tgt <- get_target_ident f.(fn_vars);
-  transf_statement_alt (Some tgt) (add_prelude_epilogue f.(fn_body))
-| _ => transf_statement_alt None f.(fn_body)
-end.
-
-Definition transf_function_alt (f: function): res function :=
-  do body <- transf_function_body_alt f;
-  OK {|
-      fn_params := f.(fn_params);
-      fn_body := body;
-
-      fn_temps := f.(fn_temps);
-      fn_vars := f.(fn_vars);
-      fn_generator := f.(fn_generator);
-
-      (*should not change*)
-      fn_return := f.(fn_return);
-      fn_callconv := f.(fn_callconv);
-      fn_blocktype := f.(fn_blocktype);
-     |}.
