stanfrontend/StanE.v
@@ -117,6 +117,7 @@ Record program := mkprogram {
   pr_defs: list (ident * globdef fundef variable);
   pr_public: list ident;
   pr_model: ident;
+  pr_target: ident;
   pr_parameters: ident;
   pr_parameters_vars: list (ident * basic);
   (* pr_parameters_vars: list ident; *)
